changed lutt_extras_ext_tmp.v; proved main lemma. 2b cleaned

proofs/itrees/lutt_extras_ext_tmp.v
@@ -1794,7 +1794,7 @@ Section Lutt_with_id.
   
 Context {hnd1 : E1 ~> execT (itree E2)}.  
 
-(* proved with axiom; easy to fix. *)
+(* MAIN: proved with axiom; easy to fix. *)
 Lemma luttNL2rutt_inr_exec_with_id (T : Type) 
   (t : itree (E1 +' E2) T) :
   lutt (fun (T0 : Type) e => ~~ is_inlB (T:=T0) e)
@@ -1904,7 +1904,14 @@ End Safe_sec1R.
 
 (*********************************************************************)
 
+Require Import it_exec_sem.
+
+(*
+Print handle_Err.
 Require Import it_sems_core.
+Print handle_Err.
+Locate handle_Err.
+*)
 
 Section Test.
 
@@ -1913,15 +1920,15 @@ Context {E: Type -> Type}.
 Definition esdflt {A} (a : A) (r : execS A) : A :=
   if r is ESok v then v else a.
 
-Let foo {E X} (d : X) (t : itree (ErrEvent +' E) X) : itree E X :=
+Let ret_dflt {E X} (d : X) (t : itree (ErrEvent +' E) X) : itree E X :=
   ITree.bind (interp_Err t) (fun x => Ret (esdflt d x)).
 
-(* ok, but trivial *)
-Lemma test1_good V1 d1 d2 
+(* basic monotonicity, with hyp about RR *)
+Lemma test_basic V1 d1 d2 
   (t1: itree (ErrEvent +' E) V1) (t2: itree (ErrEvent +' E) V1) RR :
   RR d1 d2 ->
   simple_rutt RR t1 t2 ->
-  simple_rutt RR (foo d1 t1) (foo d2 t2).
+  simple_rutt RR (ret_dflt d1 t1) (ret_dflt d2 t2).
 Proof.
   intros H H0.
   eapply simple_rutt_eutt_equiv; eauto.
@@ -1937,50 +1944,22 @@ Proof.
     destruct r2 eqn:was_r2; eauto; try (intuition auto with * ).
 Qed.
 
-Definition this_rel1 {T1 T2} (RR: T1 -> T2 -> Prop) :
+(* used to lift the return values relation *)
+Definition ok_ret_rel {T1 T2} (RR: T1 -> T2 -> Prop) :
   execS T1 -> execS T2 -> Prop :=
   fun x y => match (x, y) with
              | (ESok x', ESok y') => RR x' y'
              | _ => False end.
 
-Definition this_rel2 {T1 T2} (RR: T1 -> T2 -> Prop) :
+(* considered, but not useful *)
+Definition ok_ret_relA {T1 T2} (RR: T1 -> T2 -> Prop) :
   execS T1 -> execS T2 -> Prop :=
   fun x y => match (x, y) with
              | (ESok x', ESok y') => RR x' y'
              | (ESerror d1, ESerror d2) => eq d1 d2
              | _ => False end.
 
-(* kind of good, but admit will go through with void *)
-Lemma test2 V1 d1 d2 
-  (t1: itree (ErrEvent +' E) V1) (t2: itree (ErrEvent +' E) V1) RR :
-  @safe _ is_inlB V1 t1 ->
-  simple_rutt RR t1 t2 ->
-  simple_rutt RR (foo d1 t1) (foo d2 t2).
-Proof.
-  unfold safe, lutt.
-  intros H H0.
-  eapply simple_rutt_eutt_equiv; eauto.
-  eapply rutt2eutt in H0.
-  eapply luttNL2rutt_inr_exec_with_id in H as H1.
-  (*  destruct H as [t0 H]. *)
-  clear H.
-  eapply eqit_bind'.
-  
-  - instantiate (1 := this_rel1 RR); simpl. 
-    eapply rutt_inr2eutt_inr in H1.
-    unfold eqit_inr, eqit_img in H1.
-    unfold hnd_ext in H1.
-    instantiate (1 := handle_Err) in H1.
-    admit.
-   (*  eapply interp_exec_eutt; auto. *)
-  - intros r1 r2 H2.
-    setoid_rewrite <- eqit_Ret.
-    unfold this_rel1 in H2.
-    destruct r1 eqn:was_r1; eauto; try (intuition auto).
-    destruct r2 eqn:was_r2; eauto; try (intuition auto).
-Admitted. 
-  
-
+ 
 (* ok with void *)
 Lemma aux_eqit_lemma
   (V1 : Type)
@@ -1990,9 +1969,8 @@ Lemma aux_eqit_lemma
   (H1 : eqit (fun x : V1 => [eta eq (ESok x)]) true true t1
           (translate inr1 (interp_exec
                              (ext_exec_handler (@handle_Err void1)) t1))) :
-  eqit (this_rel1 RR)
-     true true (interp_exec ext_handle_Err t1)
-    (interp_exec ext_handle_Err t2).
+  eqit (ok_ret_rel RR) true true (interp_exec ext_handle_Err t1)
+                                 (interp_exec ext_handle_Err t2).
 Proof.
   revert H0 H1.
   revert t1 t2.
@@ -2084,8 +2062,8 @@ Proof.
   }
     
   { intros t0 t2 H H1 H2; simpl.
-    cut (gpaco2 (eqit_ (this_rel1 RR) true true Datatypes.id)
-    (eqitC (this_rel1 RR) true true) bot2 r
+    cut (gpaco2 (eqit_ (ok_ret_rel RR) true true Datatypes.id)
+    (eqitC (ok_ret_rel RR) true true) bot2 r
     (interp_exec ext_handle_Err t1)
     (interp_exec ext_handle_Err {| _observe := ot2 |})). 
     { intro K2.
@@ -2099,10 +2077,10 @@ Proof.
       }
       { reflexivity. }
       { auto. }
-      { unfold this_rel1; simpl; intros.
+      { unfold ok_ret_rel; simpl; intros.
         inv H3; auto.
       }
-      { unfold this_rel1; simpl; intros.
+      { unfold ok_ret_rel; simpl; intros.
         inv H3; auto.
       }  
     }  
@@ -2118,8 +2096,8 @@ Proof.
   }
 
   { intros t1 t0 H H1 H2; simpl.
-    cut (gpaco2 (eqit_ (this_rel1 RR) true true Datatypes.id)
-    (eqitC (this_rel1 RR) true true) bot2 r
+    cut (gpaco2 (eqit_ (ok_ret_rel RR) true true Datatypes.id)
+    (eqitC (ok_ret_rel RR) true true) bot2 r
     (interp_exec ext_handle_Err {| _observe := ot1 |})
     (interp_exec ext_handle_Err t2)).
     { intro K2.
@@ -2133,10 +2111,10 @@ Proof.
         reflexivity.
       }
       { auto. }
-      { unfold this_rel1; simpl; intros.
+      { unfold ok_ret_rel; simpl; intros.
         inv H3; auto.
       }
-      { unfold this_rel1; simpl; intros.
+      { unfold ok_ret_rel; simpl; intros.
         inv H3; auto.
       }  
     }  
@@ -2146,6 +2124,7 @@ Proof.
   } 
 Qed. 
 
+
 (* even simpler than with eqit *)
 Lemma aux_rutt_inr_lemma (VV : E = void1)
   (V1 : Type)
@@ -2154,7 +2133,7 @@ Lemma aux_rutt_inr_lemma (VV : E = void1)
   (H0 : eutt RR t1 t2)
   (H1 : rutt_inr (fun x : V1 => [eta eq (ESok x)])
                   t1 (interp_exec ext_handle_Err t1)) :
-  eqit (this_rel1 RR) true true (interp_exec ext_handle_Err t1)
+  eqit (ok_ret_rel RR) true true (interp_exec ext_handle_Err t1)
     (interp_exec ext_handle_Err t2).
 (* (H1 : rutt 
       (fun (U1 U2 : Type) (e1 : (ErrEvent +' E) U1) (e2 : E U2) =>
@@ -2213,8 +2192,8 @@ Proof.
   }
 
   { intros t0 t2 H H1 H2; simpl.
-    cut (gpaco2 (eqit_ (this_rel1 RR) true true Datatypes.id)
-    (eqitC (this_rel1 RR) true true) bot2 r
+    cut (gpaco2 (eqit_ (ok_ret_rel RR) true true Datatypes.id)
+    (eqitC (ok_ret_rel RR) true true) bot2 r
     (interp_exec ext_handle_Err t1)
     (interp_exec ext_handle_Err {| _observe := ot2 |})). 
     { intro K2.
@@ -2228,10 +2207,10 @@ Proof.
       }
       { reflexivity. }
       { auto. }
-      { unfold this_rel1; simpl; intros.
+      { unfold ok_ret_rel; simpl; intros.
         inv H3; auto.
       }
-      { unfold this_rel1; simpl; intros.
+      { unfold ok_ret_rel; simpl; intros.
         inv H3; auto.
       }  
     }  
@@ -2249,8 +2228,8 @@ Proof.
   }
 
   { intros t1 t0 H H1 H2; simpl.
-    cut (gpaco2 (eqit_ (this_rel1 RR) true true Datatypes.id)
-    (eqitC (this_rel1 RR) true true) bot2 r
+    cut (gpaco2 (eqit_ (ok_ret_rel RR) true true Datatypes.id)
+    (eqitC (ok_ret_rel RR) true true) bot2 r
     (interp_exec ext_handle_Err {| _observe := ot1 |})
     (interp_exec ext_handle_Err t2)).
     { intro K2. 
@@ -2264,10 +2243,10 @@ Proof.
         reflexivity.
       }
       { auto. }
-      { unfold this_rel1; simpl; intros.
+      { unfold ok_ret_rel; simpl; intros.
         inv H3; auto.
       }
-      { unfold this_rel1; simpl; intros.
+      { unfold ok_ret_rel; simpl; intros.
         inv H3; auto.
       }  
     }  
@@ -2296,7 +2275,7 @@ Lemma aux_deep_rutt_lemma (VV : E = void1)
       (fun U1 U2 : Type =>
               fun=> (fun u1 : U1 => fun=> [eta JMeq u1 (B:=U2)]))
       (fun x : V1 => [eta eq (ESok x)]) t1 (interp_exec ext_handle_Err t1)) :
-  eqit (this_rel1 RR) true true (interp_exec ext_handle_Err t1)
+  eqit (ok_ret_rel RR) true true (interp_exec ext_handle_Err t1)
                                 (interp_exec ext_handle_Err t2).
 Proof.
   revert H0 H1.
@@ -2350,8 +2329,8 @@ Proof.
   }
 
   { intros t0 t2 H H1 H2; simpl.
-    cut (gpaco2 (eqit_ (this_rel1 RR) true true Datatypes.id)
-    (eqitC (this_rel1 RR) true true) bot2 r
+    cut (gpaco2 (eqit_ (ok_ret_rel RR) true true Datatypes.id)
+    (eqitC (ok_ret_rel RR) true true) bot2 r
     (interp_exec ext_handle_Err t1)
     (interp_exec ext_handle_Err {| _observe := ot2 |})). 
     { intro K2.
@@ -2365,10 +2344,10 @@ Proof.
       }
       { reflexivity. }
       { auto. }
-      { unfold this_rel1; simpl; intros.
+      { unfold ok_ret_rel; simpl; intros.
         inv H3; auto.
       }
-      { unfold this_rel1; simpl; intros.
+      { unfold ok_ret_rel; simpl; intros.
         inv H3; auto.
       }  
     }  
@@ -2386,8 +2365,8 @@ Proof.
   }
 
   { intros t1 t0 H H1 H2; simpl.
-    cut (gpaco2 (eqit_ (this_rel1 RR) true true Datatypes.id)
-    (eqitC (this_rel1 RR) true true) bot2 r
+    cut (gpaco2 (eqit_ (ok_ret_rel RR) true true Datatypes.id)
+    (eqitC (ok_ret_rel RR) true true) bot2 r
     (interp_exec ext_handle_Err {| _observe := ot1 |})
     (interp_exec ext_handle_Err t2)).
     { intro K2. 
@@ -2401,10 +2380,10 @@ Proof.
         reflexivity.
       }
       { auto. }
-      { unfold this_rel1; simpl; intros.
+      { unfold ok_ret_rel; simpl; intros.
         inv H3; auto.
       }
-      { unfold this_rel1; simpl; intros.
+      { unfold ok_ret_rel; simpl; intros.
         inv H3; auto.
       }  
     }  
@@ -2418,46 +2397,18 @@ Proof.
 Qed.  
 
 
-(* kind of good, but admit will go through with void *)
-Lemma test2_rev (VV : E = void1) V1 d1 d2 
-  (t1: itree (ErrEvent +' E) V1) (t2: itree (ErrEvent +' E) V1) RR :
-  @safe _ is_inlB V1 t1 ->
-  simple_rutt RR t1 t2 ->
-  simple_rutt RR (foo d1 t1) (foo d2 t2).
-Proof.
-  unfold safe, lutt.
-  intros H H0.
-  eapply simple_rutt_eutt_equiv; eauto.
-  eapply rutt2eutt in H0.
-  eapply luttNL2rutt_inr_exec_with_id in H.
-  eapply eqit_bind'.
-  
-  - instantiate (1 := this_rel1 RR); simpl.
-    eapply aux_rutt_inr_lemma; auto.
-    exact H.
-  - intros r1 r2 H1.
-    setoid_rewrite <- eqit_Ret.
-    unfold this_rel1 in H1.
-    destruct r1 eqn:was_r1; eauto; try (intuition auto).
-    destruct r2 eqn:was_r2; eauto; try (intuition auto).
-Qed.
-
-
-(************************************************************************)
-
-
-(* ok with void *)
-Lemma xxx 
+(* identical to the previous one: the precondition can be abstracted *)
+Lemma aux_abs_rutt_lemma (VV : E = void1)
+  (PreR: prerel (ErrEvent +' E) E)
+  (PostR: postrel (ErrEvent +' E) E)
   (V1 : Type)
-  (t1 t2 : itree (ErrEvent +' void1) V1)
+  (RRel: V1 -> execS V1 -> Prop)
+  (t1 t2 : itree (ErrEvent +' E) V1)
   (RR : V1 -> V1 -> Prop)
   (H0 : eutt RR t1 t2)
-  (H1 : rutt_inr (fun x : V1 => [eta eq (ESok x)])
-                  t1 (interp_exec ext_handle_Err t1)) :
-(* eqit (fun x : V1 => [eta eq (ESok x)]) true true t1
-      (translate inr1 (interp_exec (ext_exec_handler (@handle_Err E)) t1))) : *)
-  eqit (this_rel1 RR) true true (interp_exec ext_handle_Err t1)
-    (interp_exec ext_handle_Err t2).
+  (H1 : rutt PreR PostR RRel t1 (interp_exec ext_handle_Err t1)) :
+  eqit (ok_ret_rel RR) true true (interp_exec ext_handle_Err t1)
+                                (interp_exec ext_handle_Err t2).
 Proof.
   revert H0 H1.
   revert t1 t2.
@@ -2486,184 +2437,133 @@ Proof.
     econstructor.
     gfinal; left.
     eapply CIH; eauto.
-    unfold rutt_inr, rutt_img in H1. 
+    unfold rutt_inr, rutt_img in *.
     setoid_rewrite interp_exec_tau in H1.
     setoid_rewrite tau_eutt in H1; auto.
   }
   { intros t1 t2 H H0 H1; simpl.
+
+(*    generalize H1; intro Hcopy.  *)
+    
     setoid_rewrite interp_exec_vis.
-    unfold rutt_inr, rutt_img in H1.
     setoid_rewrite interp_exec_vis in H1.
-    guclo eqit_clo_bind.
-    econstructor 1 with (RU := eq).
+
+    destruct e as [e1 | e1] eqn: was_e ; simpl in *; simpl.    
+
+    { destruct e1; simpl in *.
+      setoid_rewrite bind_ret_l in H1.
+      punfold H1; red in H1.
+      dependent destruction H1.
+    }  
+
+    dependent destruction VV.
+    destruct e1.
+  }
+
+  { intros t0 t2 H H1 H2; simpl.
+    cut (gpaco2 (eqit_ (ok_ret_rel RR) true true Datatypes.id)
+    (eqitC (ok_ret_rel RR) true true) bot2 r
+    (interp_exec ext_handle_Err t1)
+    (interp_exec ext_handle_Err {| _observe := ot2 |})). 
+    { intro K2.
+      guclo eqit_clo_trans.
+      econstructor.
+      { instantiate (2:= eq).
+        instantiate (1:= (interp_exec ext_handle_Err t1)).
+        setoid_rewrite interp_exec_tau.
+        setoid_rewrite tau_euttge.
+        reflexivity.
+      }
+      { reflexivity. }
+      { auto. }
+      { unfold ok_ret_rel; simpl; intros.
+        inv H3; auto.
+      }
+      { unfold ok_ret_rel; simpl; intros.
+        inv H3; auto.
+      }  
+    }  
+
+    setoid_rewrite (itree_eta t1).
+    eapply IHeqitF.
     reflexivity.
+    eexact H1.
 
-    rename u into U.
-    intros u1 u2 H2.
-    inv H2.
-    gfinal; right.
-    destruct u2 as [u1 | d1] eqn: was_u2.
+    eapply rutt_inv_Tau_l.
+    eapply rutt_inv_Tau_r.
+    setoid_rewrite (itree_eta t1) in H2.
+    setoid_rewrite interp_exec_tau in H2.
+    auto.
+  }
+
+  { intros t1 t0 H H1 H2; simpl.
+    cut (gpaco2 (eqit_ (ok_ret_rel RR) true true Datatypes.id)
+    (eqitC (ok_ret_rel RR) true true) bot2 r
+    (interp_exec ext_handle_Err {| _observe := ot1 |})
+    (interp_exec ext_handle_Err t2)).
+    { intro K2. 
+      guclo eqit_clo_trans.
+      econstructor.
+      { reflexivity. }
+      { instantiate (2:= eq).
+        instantiate (1:= (interp_exec ext_handle_Err t2)).
+        setoid_rewrite interp_exec_tau.
+        setoid_rewrite tau_euttge.
+        reflexivity.
+      }
+      { auto. }
+      { unfold ok_ret_rel; simpl; intros.
+        inv H3; auto.
+      }
+      { unfold ok_ret_rel; simpl; intros.
+        inv H3; auto.
+      }  
+    }  
     
-    { pstep; red.
-      econstructor. right.
-      eapply CIH.
-      specialize (REL u1); pclearbot; auto.
-      unfold ext_exec_handler.
+    setoid_rewrite (itree_eta t2).
+    eapply IHeqitF.
+    eexact H.
+    reflexivity.
+    auto.
+  }
+Qed.  
 
-Check @interp_exec_translate.
-      admit.
-    }
-
-    pstep; red. econstructor.
-
-    destruct e as [e1 | e2] eqn:was_e;  simpl in *.
-
-    (* error case: should go through *)
-    punfold H1; red in H1.
-    dependent destruction H1.
-    destruct H1 as [hh H1].
-    dependent destruction hh.
-    simpl in H1.
-    inversion H1.
-
-    admit.
-
-    destruct e2.
-
-Admitted. 
-    
-
-(* best initial try: ok with void *)
-Lemma xxx0 
-  (V1 : Type)
-  (t1 t2 : itree (ErrEvent +' void1) V1)
-  (RR : V1 -> V1 -> Prop)
-  (H0 : eutt RR t1 t2)
-  (H1 : eqit (fun x : V1 => [eta eq (ESok x)]) true true t1
-      (translate inr1 (interp_exec (ext_exec_handler (@handle_Err void1)) t1))) :
-  eqit
-    (fun x y : execS V1 =>
-     match x with
-     | ESok x' =>
-         match y with
-         | ESok y' => RR x' y'
-         | @ESerror _ _ => False
-         end
-     | @ESerror _ _ => False
-     end) true true (interp_exec ext_handle_Err t1)
-    (interp_exec ext_handle_Err t2).
+Lemma test2_abs (VV : E = void1) V1 d1 d2 
+  (t1: itree (ErrEvent +' E) V1) (t2: itree (ErrEvent +' E) V1) RR :
+  @safe _ is_inlB V1 t1 ->
+  simple_rutt RR t1 t2 ->
+  simple_rutt RR (ret_dflt d1 t1) (ret_dflt d2 t2).
 Proof.
-  revert H0 H1.
-  revert t1 t2.
-  ginit.
-  gcofix CIH.
-  intros t1 t2 H0 H1.
-  setoid_rewrite (itree_eta t2).
-  setoid_rewrite (itree_eta t2) in H0.
-  setoid_rewrite (itree_eta t1).
-  setoid_rewrite (itree_eta t1) in H0.
-  setoid_rewrite (itree_eta t1) in H1.  
-  remember (observe t1) as ot1.
-  remember (observe t2) as ot2.
-  punfold H0. red in H0.
-  simpl in *.
-  hinduction H0 before CIH.
-
-  { intros t1 t2 H H0 H1; simpl.
-    setoid_rewrite interp_exec_Ret.
-    gstep; red.
-    econstructor; eauto.
-  }
-  { intros t1 t2 H H0 H1; simpl.
-    setoid_rewrite interp_exec_tau.  
-    gstep; red; pclearbot.
-    econstructor.
-    gfinal; left.
-    eapply CIH; eauto.
-    setoid_rewrite interp_exec_tau in H1.
-    setoid_rewrite translate_tau in H1.
-    setoid_rewrite tau_eutt in H1; auto.
-  }
-  { intros t1 t2 H H0 H1; simpl.
-    setoid_rewrite interp_exec_vis.
-    setoid_rewrite interp_exec_vis in H1.
-    setoid_rewrite translate_bind in H1.    
-    guclo eqit_clo_bind.
-    econstructor 1 with (RU := eq).
-    reflexivity.
-
-    rename u into U.
-    intros u1 u2 H2.
-    inv H2.
-    gfinal; right.
-    destruct u2 as [u1 | d1] eqn: was_u2.
-    
-    { pstep; red.
-      econstructor. right.
-      eapply CIH.
-      specialize (REL u1); pclearbot; auto.
-      unfold ext_exec_handler.
-
-Check @interp_exec_translate.
-      admit.
-    }
-
-    pstep; red. econstructor.
-
-    destruct e as [e1 | e2] eqn:was_e;  simpl in *.
-
-    (* error case: should go through *)
-    eapply eqit_flip in H1.
-    eapply eqit_inv_bind_vis in H1.
-    unfold handle_Err in H1; simpl in H1.
-    destruct e1; simpl in *.
-    admit.
-
-    inversion e2.
-Admitted. 
+  unfold safe, lutt.
+  intros H H0.
+  eapply simple_rutt_eutt_equiv; eauto.
+  eapply rutt2eutt in H0.
+  eapply luttNL2rutt_inr_exec_with_id in H.
+  eapply eqit_bind'.  
+  - instantiate (1 := ok_ret_rel RR); simpl.
+    eapply aux_abs_rutt_lemma; eauto.
+  - intros r1 r2 H1.
+    setoid_rewrite <- eqit_Ret.
+    unfold ok_ret_rel in H1.
+    destruct r1 eqn:was_r1; eauto; try (intuition auto).
+    destruct r2 eqn:was_r2; eauto; try (intuition auto).
+Qed.
 
 
-Lemma xxx111 
+(* identical to the previous one: the precondition can be abstracted *)
+Lemma aux_gen_rutt_lemma 
+  (PreR: prerel E E)
+  (PostR: postrel E E)
   (V1 : Type)
+  (RRel: execS V1 -> execS V1 -> Prop)
+  (RRel_hyp: forall e0, RRel (ESerror V1 e0) (ESerror V1 e0) -> False)
+  (PostR_hyp: forall T e1 v1, PostR T T e1 v1 e1 v1)
   (t1 t2 : itree (ErrEvent +' E) V1)
   (RR : V1 -> V1 -> Prop)
   (H0 : eutt RR t1 t2)
-  (H1 : rutt
-      (fun (U1 U2 : Type) (e1 : (ErrEvent +' E) U1) (e2 : E U2) =>
-              match e1 with
-              | inl1 _ => False 
-              | inr1 _ => exists h : U2 = U1,
-                    e1 = eq_rect U2 (ErrEvent +' E) (inr1 e2) U1 h end) 
-      (fun U1 U2 : Type =>
-       fun e1 (u1 : U1) e2 u2 =>
-         ((forall (U3: Type) (h : execS U3 = U1),
-              (exists d1,
-               u1 = eq_rect (execS U3) id (ESerror _ d1) U1 h)) -> False) /\
-               JMeq u1 u2)
-      (fun x : V1 => [eta eq (ESok x)]) t1 (interp_exec ext_handle_Err t1)) :
-  eqit (this_rel1 RR) true true (interp_exec ext_handle_Err t1)
-                                (interp_exec ext_handle_Err t2).
-Proof.
-  Abort.
-
-Print postrel.
-
-
-(* experiment *)
-Lemma xxx133 (Spec : postrel (ErrEvent +' E) E)
-  (V1 : Type)
-  (t1 t2 : itree (ErrEvent +' E) V1)
-  (RR : V1 -> V1 -> Prop)
-  (H0 : eutt RR t1 t2)
-  (H1 : rutt
-      (fun (U1 U2 : Type) (e1 : (ErrEvent +' E) U1) (e2 : E U2) =>
-              match e1 with
-              | inl1 _ => False 
-              | inr1 _ => exists h : U2 = U1,
-                    e1 = eq_rect U2 (ErrEvent +' E) (inr1 e2) U1 h end) 
-      Spec 
-      (fun x : V1 => [eta eq (ESok x)]) t1 (interp_exec ext_handle_Err t1)) :
-  eqit (this_rel1 RR) true true (interp_exec ext_handle_Err t1)
+  (H1 : rutt PreR PostR RRel (interp_exec ext_handle_Err t1)
+                             (interp_exec ext_handle_Err t1)) :
+  eqit (ok_ret_rel RR) true true (interp_exec ext_handle_Err t1)
                                 (interp_exec ext_handle_Err t2).
 Proof.
   revert H0 H1.
@@ -2708,84 +2608,112 @@ Proof.
       setoid_rewrite bind_ret_l in H1.
       punfold H1; red in H1.
       dependent destruction H1.
+      eapply RRel_hyp in H1; intuition.
     }  
 
+    unfold lift_ktree_ in H1.
     setoid_rewrite bind_vis in H1.
-    punfold H1. red in H1.
-    dependent destruction H1.
-    
-    guclo eqit_clo_bind.
-    econstructor 1 with (RU := eq).
-    reflexivity.
-
-    rename u into U.
-    intros u1 u2 H3.
-    inv H3.
-    destruct u2 eqn: was_u2; simpl.
-
-    {   
-      gstep; red.
-      econstructor.
-      gfinal; left.
-      eapply CIH.
-      specialize (REL u); pclearbot; auto.
-
-      specialize (H2 u u).
-      assert (Spec U U (inr1 e1) u e1 u) as K1.
-      { admit. }
-      specialize (H2 K1); pclearbot.
-      setoid_rewrite bind_ret_l_Eq in H2.
-      setoid_rewrite <- tau_euttge.
-      eapply rutt_cong_eutt.
-      eexact H2.
-      setoid_rewrite tau_eutt; reflexivity.
-    }
-
-    have my_u : U.
-    { admit. }
-    specialize (H2 my_u my_u).
-     
-    inv was_u2.
-    unfold ext_handle_Err; simpl.
+    punfold H1; red in H1.
+    setoid_rewrite bind_vis.
     gstep; red.
     econstructor.
-    unfold this_rel1.
+    intro v1.
+    unfold Datatypes.id; simpl.
+    dependent destruction H1.
 
-Admitted.     
-(*
-    
-    destruct e as [e1 | e1] eqn: was_e ; simpl in *; simpl.    
+    specialize (H2 v1 v1).
+    assert (PostR u u e1 v1 e1 v1) as K2.
+    { eapply PostR_hyp; auto. }
+   
+    setoid_rewrite bind_ret_l_Eq.
+    setoid_rewrite bind_ret_l_Eq in H2.
 
-    { destruct e1; simpl in *.
-      setoid_rewrite bind_ret_l in H1.
-      punfold H1; red in H1.
-      dependent destruction H1.
-    }  
+    cut (gpaco2 (eqit_ (ok_ret_rel RR) true true id)
+                (eqitC (ok_ret_rel RR) true true) r r
+                (interp_exec ext_handle_Err (k1 v1))
+                (interp_exec ext_handle_Err (k2 v1))).
+    { intro K3.
+      guclo eqit_clo_trans.
+      econstructor.
+      { instantiate (2:= eq).
+        instantiate (1:= (interp_exec ext_handle_Err (k1 v1))).
+        setoid_rewrite tau_euttge.
+        reflexivity.
+      }
+      { instantiate (2:= eq).
+        instantiate (1:= (interp_exec ext_handle_Err (k2 v1))).
+        setoid_rewrite tau_euttge.
+        reflexivity. }
+      { auto. }
+      { unfold ok_ret_rel; simpl; intros.
+        inv H3; auto.
+      }
+      { unfold ok_ret_rel; simpl; intros.
+        inv H3; auto.
+      }  
+    }
 
-    setoid_rewrite bind_vis in H1.
-    punfold H1. red in H1.
-*)
+    gfinal. left.
+    eapply CIH.
+    specialize (REL v1); pclearbot.
+    auto.
+
+    specialize (H2 K2); pclearbot.
+    eapply rutt_inv_Tau_l in H2.
+    eapply rutt_inv_Tau_r in H2.
+    auto.
+  }
+
+  { intros t0 t2 H H1 H2; simpl.
+    cut (gpaco2 (eqit_ (ok_ret_rel RR) true true Datatypes.id)
+    (eqitC (ok_ret_rel RR) true true) bot2 r
+    (interp_exec ext_handle_Err t1)
+    (interp_exec ext_handle_Err {| _observe := ot2 |})). 
+    { intro K2.
+      setoid_rewrite interp_exec_tau.
+      setoid_rewrite tau_euttge; auto.
+    }
+    setoid_rewrite (itree_eta t1).
+    eapply IHeqitF; eauto.
+    eapply rutt_inv_Tau_l.
+    eapply rutt_inv_Tau_r.
+    setoid_rewrite (itree_eta t1) in H2.
+    setoid_rewrite interp_exec_tau in H2.
+    auto.
+  }
+
+  { intros t1 t0 H H1 H2; simpl.
+    cut (gpaco2 (eqit_ (ok_ret_rel RR) true true Datatypes.id)
+    (eqitC (ok_ret_rel RR) true true) bot2 r
+    (interp_exec ext_handle_Err {| _observe := ot1 |})
+    (interp_exec ext_handle_Err t2)).
+    { intro K2. 
+      setoid_rewrite interp_exec_tau.
+      setoid_rewrite tau_euttge; auto.
+    }
+ 
+    setoid_rewrite (itree_eta t2).
+    eapply IHeqitF; eauto.
+  }
+Qed.
 
 
-(* older *)
-Lemma xxx 
+
+(* identical to the previous one: the precondition can be abstracted *)
+Lemma aux_gen_rutt_lemma2 
+  (PreR: prerel E E)
+  (PostR: postrel E E)
   (V1 : Type)
+  (RRel: execS V1 -> execS V1 -> Prop)
+  (RRel_hyp: forall e0, RRel (ESerror V1 e0) (ESerror V1 e0) -> False)
+  (PostR_hyp: forall T e1 v1, PostR T T e1 v1 e1 v1)
   (t1 t2 : itree (ErrEvent +' E) V1)
   (RR : V1 -> V1 -> Prop)
   (H0 : eutt RR t1 t2)
-  (H1 : eqit (fun x : V1 => [eta eq (ESok x)]) true true t1
-      (translate inr1 (interp_exec (ext_exec_handler (@handle_Err E)) t1))) :
-  eqit
-    (fun x y : execS V1 =>
-     match x with
-     | ESok x' =>
-         match y with
-         | ESok y' => RR x' y'
-         | @ESerror _ _ => False
-         end
-     | @ESerror _ _ => False
-     end) true true (interp_exec ext_handle_Err t1)
-    (interp_exec ext_handle_Err t2).
+  (H1 : rutt PreR PostR RRel (interp_exec ext_handle_Err t1)
+                             (interp_exec ext_handle_Err t2)) :
+  eqit (ok_ret_rel RR) true true (interp_exec ext_handle_Err t1)
+                                (interp_exec ext_handle_Err t2).
 Proof.
   revert H0 H1.
   revert t1 t2.
@@ -2796,7 +2724,8 @@ Proof.
   setoid_rewrite (itree_eta t2) in H0.
   setoid_rewrite (itree_eta t1).
   setoid_rewrite (itree_eta t1) in H0.
-  setoid_rewrite (itree_eta t1) in H1.  
+  setoid_rewrite (itree_eta_ t1) in H1.  
+  setoid_rewrite (itree_eta_ t2) in H1.  
   remember (observe t1) as ot1.
   remember (observe t2) as ot2.
   punfold H0. red in H0.
@@ -2814,47 +2743,605 @@ Proof.
     econstructor.
     gfinal; left.
     eapply CIH; eauto.
+    unfold rutt_inr, rutt_img in *.
     setoid_rewrite interp_exec_tau in H1.
-    setoid_rewrite translate_tau in H1.
     setoid_rewrite tau_eutt in H1; auto.
   }
   { intros t1 t2 H H0 H1; simpl.
+
     setoid_rewrite interp_exec_vis.
     setoid_rewrite interp_exec_vis in H1.
-    setoid_rewrite translate_bind in H1.    
-    guclo eqit_clo_bind.
-    econstructor 1 with (RU := eq).
-    reflexivity.
 
-    intros.
-    inv H2.
-    gfinal; right.
-    destruct u2 as [u1 | u2].
-    pstep; red.
-    econstructor. right.
+    destruct e as [e1 | e1] eqn: was_e ; simpl in *; simpl.    
+
+    { destruct e1; simpl in *.
+      setoid_rewrite bind_ret_l in H1.
+      punfold H1; red in H1.
+      dependent destruction H1.
+      eapply RRel_hyp in H1; intuition.
+    }  
+
+    unfold lift_ktree_ in H1.
+    setoid_rewrite bind_vis in H1.
+    punfold H1; red in H1.
+    setoid_rewrite bind_vis.
+    gstep; red.
+    econstructor.
+    intro v1.
+    unfold Datatypes.id; simpl.
+    dependent destruction H1.
+
+    specialize (H2 v1 v1).
+    assert (PostR u u e1 v1 e1 v1) as K2.
+    { eapply PostR_hyp; auto. }
+   
+    setoid_rewrite bind_ret_l_Eq.
+    setoid_rewrite bind_ret_l_Eq in H2.
+    specialize (H2 K2); pclearbot.
+    
+    cut (gpaco2 (eqit_ (ok_ret_rel RR) true true id)
+                (eqitC (ok_ret_rel RR) true true) r r
+                (interp_exec ext_handle_Err (k1 v1))
+                (interp_exec ext_handle_Err (k2 v1))).
+    { intro K3.
+      guclo eqit_clo_trans.
+      econstructor.
+      { instantiate (2:= eq).
+        instantiate (1:= (interp_exec ext_handle_Err (k1 v1))).
+        setoid_rewrite tau_euttge.
+        reflexivity.
+      }
+      { instantiate (2:= eq).
+        instantiate (1:= (interp_exec ext_handle_Err (k2 v1))).
+        setoid_rewrite tau_euttge.
+        reflexivity. }
+      { auto. }
+      { unfold ok_ret_rel; simpl; intros.
+        inv H3; auto.
+      }
+      { unfold ok_ret_rel; simpl; intros.
+        inv H3; auto.
+      }  
+    }
+
+    gfinal. left.
     eapply CIH.
-    specialize (REL u1); pclearbot; auto.
-    admit.
-    pstep; red. econstructor.
-    setoid_rewrite eqit_Ret.
-    
-    setoid_rewrite <- tau_eutt.    
-    
-    instantiate (2 := (fun x y : execS u =>
-     match x with
-     | ESok x' =>
-         match y with
-         | ESok y' => RR x' y'
-         | @ESerror _ _ => False
-         end
-     | @ESerror _ _ => False
-     end)).
-    
-    gstep; red; simpl.
-    
-    
-Admitted.   
+    specialize (REL v1); pclearbot.
+    auto.
 
+    eapply rutt_inv_Tau_l in H2.
+    eapply rutt_inv_Tau_r in H2.
+    auto.
+  }
+
+  { intros t0 t2 H H1 H2; simpl.
+    cut (gpaco2 (eqit_ (ok_ret_rel RR) true true Datatypes.id)
+    (eqitC (ok_ret_rel RR) true true) bot2 r
+    (interp_exec ext_handle_Err t1)
+    (interp_exec ext_handle_Err {| _observe := ot2 |})). 
+    { intro K2.
+      setoid_rewrite interp_exec_tau.
+      setoid_rewrite tau_euttge; auto.
+    }
+    setoid_rewrite (itree_eta t1).
+    eapply IHeqitF; eauto.
+    setoid_rewrite tau_euttge in H2.
+    setoid_rewrite (itree_eta t1) in H2. auto.
+  }
+
+  { intros t1 t0 H H1 H2; simpl.
+    cut (gpaco2 (eqit_ (ok_ret_rel RR) true true Datatypes.id)
+    (eqitC (ok_ret_rel RR) true true) bot2 r
+    (interp_exec ext_handle_Err {| _observe := ot1 |})
+    (interp_exec ext_handle_Err t2)).
+    { intro K2. 
+      setoid_rewrite interp_exec_tau.
+      setoid_rewrite tau_euttge; auto.
+    }
+    setoid_rewrite tau_euttge in H2. 
+    setoid_rewrite (itree_eta t2) in H2.
+    setoid_rewrite (itree_eta t2).
+    eapply IHeqitF; eauto.
+  }
+Qed.
+
+
+(* kind of good, but admit will go through with void *)
+Lemma test2_rev (VV : E = void1) V1 d1 d2 
+  (t1: itree (ErrEvent +' E) V1) (t2: itree (ErrEvent +' E) V1) RR :
+  @safe _ is_inlB V1 t1 ->
+  simple_rutt RR t1 t2 ->
+  simple_rutt RR (ret_dflt d1 t1) (ret_dflt d2 t2).
+Proof.
+  unfold safe, lutt.
+  intros H H0.
+  eapply simple_rutt_eutt_equiv; eauto.
+  eapply rutt2eutt in H0.
+  eapply luttNL2rutt_inr_exec_with_id in H.
+  eapply eqit_bind'.
+  
+  - instantiate (1 := ok_ret_rel RR); simpl.
+    eapply aux_rutt_inr_lemma; auto.
+    exact H.
+  - intros r1 r2 H1.
+    setoid_rewrite <- eqit_Ret.
+    unfold ok_ret_rel in H1.
+    destruct r1 eqn:was_r1; eauto; try (intuition auto).
+    destruct r2 eqn:was_r2; eauto; try (intuition auto).
+Qed.
+
+
+Definition ok_rutt T1 T2 RR
+  (t1 : itree (ErrEvent +' E) T1)
+  (t2 : itree (ErrEvent +' E) T2) : Prop := 
+  rutt (fun U1 U2 (e1: E U1) (e2: E U2) =>
+          exists h : U2 = U1, e1 = eq_rect U2 E e2 U1 h)
+       (fun U1 U2 (e1: E U1) (u1: U1) (e2: E U2) (u2: U2) => JMeq u1 u2)
+       (fun r1 r2 => match (r1, r2) with
+                     | (ESok v1, ESok v2) => RR v1 v2
+                     | _ => False end)
+       (interp_exec ext_handle_Err t1) (interp_exec ext_handle_Err t2). 
+
+(*
+Definition ok_rutt T1 T2 RR
+  (t1 : itree (ErrEvent +' E) T1)
+  (t2 : itree (ErrEvent +' E) T2) : Prop := 
+  rutt (fun U1 U2 (e1: E U1) (e2: E U2) =>
+          exists h : U2 = U1, e1 = eq_rect U2 E e2 U1 h)
+       (fun U1 U2 (e1: E U1) (u1: U1) (e2: E U2) (u2: U2) => JMeq u1 u2)
+       (R_eq (fun x => match x with | ESok _ => True | _ => False end))
+       (interp_exec ext_handle_Err t1) (interp_exec ext_handle_Err t2). 
+*)
+
+Definition ok_deep_rutt E0 T1 T2 RR
+  (t1 : itree E0 T1) (t2 : itree E0 T2) : Prop := 
+  rutt (fun U1 U2 (e1: E0 U1) (e2: E0 U2) =>
+          exists h : U2 = U1, e1 = eq_rect U2 E0 e2 U1 h)       
+       (fun U1 U2 (e1: E0 U1) (u1: U1) (e2: E0 U2) (u2: U2) =>
+          (exists U3 (h2: U1 = execS U3), 
+                 match eq_rect U1 id u1 (execS U3) h2 with
+                 | ESok v => JMeq u1 u2
+                 | ESerror d => False end)
+          \/ (forall U3, ~ (U1 = execS U3) /\ JMeq u1 u2)) RR t1 t2. 
+
+(*
+Lemma ok_deep_rutt2eutt E0 T1 T2 RR 
+  (t1: itree E0 T1) (t2: itree E0 T2) :
+ @ok_deep_rutt E0 T1 T2 RR t1 t2 -> eutt RR t1 t2.
+Proof.
+  revert t1 t2.
+  ginit; gcofix CIH.
+  unfold simple_rutt.
+  intros t1 t2 H.
+  rewrite (itree_eta t1).
+  rewrite (itree_eta t2).
+  punfold H; red in H; simpl in H.   
+  remember (observe t1) as ot1.
+  remember (observe t2) as ot2.
+  hinduction H before CIH.
+  
+  { intros t1 t2 H0 H1.
+    gstep; red; simpl.
+    econstructor; auto.
+  }
+  { intros t1 t2 H0 H1.
+    gstep; red; simpl; pclearbot.
+    econstructor; eauto.
+    gfinal; left.
+    eapply CIH; auto.
+  }
+  { intros t1 t2 H1 H2.
+    gstep; red; simpl.
+    destruct H as [ee HA].
+    dependent destruction ee.
+    simpl in HA. inv HA.  
+    econstructor.
+    intros v; unfold Datatypes.id; simpl.
+    gfinal; left; pclearbot.
+    eapply CIH; auto; simpl.
+    eapply H0; auto.
+  }
+  { intros t1' t2 H0 H1.
+    guclo eqit_clo_trans.
+    econstructor 1 with (RR1 := eq) (RR2:= eq); auto.
+    instantiate (1:= t1).
+    eapply eqit_Tau_l; reflexivity.
+    reflexivity.
+    setoid_rewrite (itree_eta t1).
+    pclearbot; eapply IHruttF; auto.
+    exact H1.
+    intros; inv H2; auto.
+    intros; inv H2; auto.
+  }
+  { intros t1 t2' H0 H1.
+    guclo eqit_clo_trans.
+    econstructor 1 with (RR1 := eq) (RR2:= eq); auto.
+    3: { eapply IHruttF; try reflexivity; eauto. }
+    { inv H0; simpl.
+      setoid_rewrite (itree_eta t1) at 2; reflexivity.
+    }  
+    { eapply eqit_Tau_l.
+      setoid_rewrite (itree_eta t2) at 1; reflexivity.
+    }  
+    { intros; inv H2; auto. }
+    { intros; inv H2; auto. }
+  }
+Qed.  
+*)  
+ 
+Lemma test2_gen_ok V1 d1 d2 
+  (t1: itree (ErrEvent +' E) V1) (t2: itree (ErrEvent +' E) V1) RR :
+  (*  @safe _ is_inlB V1 t1 -> *)
+  ok_rutt RR t1 t1 ->
+  simple_rutt RR t1 t2 ->
+  simple_rutt RR (ret_dflt d1 t1) (ret_dflt d2 t2).
+Proof.
+  unfold safe, lutt.
+  intros H H0.
+  eapply simple_rutt_eutt_equiv; eauto.
+  eapply rutt2eutt in H0.
+  eapply eqit_bind'.
+  
+  - instantiate (1 := ok_ret_rel RR); simpl.
+    eapply aux_gen_rutt_lemma in H; eauto.                                   
+  - intros r1 r2 H1.
+    setoid_rewrite <- eqit_Ret.
+    unfold ok_ret_rel in H1.
+    destruct r1 eqn:was_r1; eauto; try (intuition auto).
+    destruct r2 eqn:was_r2; eauto; try (intuition auto).
+Qed.
+
+Lemma test2_gen_ok2 V1 d1 d2 
+  (t1: itree (ErrEvent +' E) V1) (t2: itree (ErrEvent +' E) V1) RR :
+  (*  @safe _ is_inlB V1 t1 -> *)
+  ok_rutt RR t1 t2 ->
+  simple_rutt RR t1 t2 ->
+  simple_rutt RR (ret_dflt d1 t1) (ret_dflt d2 t2).
+Proof.
+  unfold safe, lutt.
+  intros H H0.
+  eapply simple_rutt_eutt_equiv; eauto.
+  eapply rutt2eutt in H0.
+  eapply eqit_bind'.
+  
+  - instantiate (1 := ok_ret_rel RR); simpl.
+    eapply aux_gen_rutt_lemma2 in H; eauto.                                   
+  - intros r1 r2 H1.
+    setoid_rewrite <- eqit_Ret.
+    unfold ok_ret_rel in H1.
+    destruct r1 eqn:was_r1; eauto; try (intuition auto).
+    destruct r2 eqn:was_r2; eauto; try (intuition auto).
+Qed.
+
+
+Lemma rutt2ok_rutt V1 (t1 t2: itree (ErrEvent +' E) V1) RR :
+  (*  @safe _ is_inlB V1 t1 -> *)
+  rutt (REv_eq (fun (T : Type) (e : (ErrEvent +' E) T) => ~~ is_inlB e))
+       (RAns_eq (fun T : Type => fun=> TrueP)) RR t1 t2 ->
+  ok_rutt RR t1 t2.
+Proof.
+  revert t1 t2.
+  ginit. gcofix CIH.
+  intros t1 t2 H.
+  setoid_rewrite (itree_eta t1) in H.
+  setoid_rewrite (itree_eta t2) in H.
+  setoid_rewrite (itree_eta t1).
+  setoid_rewrite (itree_eta t2).
+  punfold H; red in H.
+  remember (observe t1) as ot1.
+  remember (observe t2) as ot2.
+  simpl in H.
+  hinduction H before CIH.
+  { intros t1 t2 H0.
+    setoid_rewrite interp_exec_ret.
+    gstep; red.
+    econstructor; auto.
+  }
+  { intros t1 t2 H0 H1; pclearbot.
+    setoid_rewrite interp_exec_tau.
+    gstep; red.
+    econstructor; eauto.
+    gfinal; left.
+    eapply CIH; eauto.
+  }
+  { intros t1 t2 H1 H2.
+    setoid_rewrite interp_exec_vis.
+    (* check this *)
+    eapply gpaco2_uclo; [|eapply rutt_clo_bind|]; eauto with paco.
+    econstructor 1 with
+      (RU := (fun (r1: execS A) (r2: execS B) =>
+                     match (r1, r2) with
+                     | (ESok v1, ESok v2) => JMeq v1 v2
+                     | _ => False end)).
+    { destruct e1; simpl.
+      { unfold REv_eq in H; simpl in H; intuition. }
+      { destruct e2.
+        { unfold REv_eq in H; simpl in H; intuition.
+          destruct H4 as [hh H4].
+          dependent destruction hh; simpl in *; try discriminate.
+        }
+        simpl.
+        pstep; red.
+        econstructor.
+        { unfold REv_eq in H; simpl in *.
+          destruct H as [_ [hh H]].
+          dependent destruction hh; simpl in *.
+          dependent destruction H.
+          exists erefl; simpl; auto.
+        }
+        { intros a b hh.
+          dependent destruction hh.
+          simpl. left.
+          pstep; red.
+          econstructor. auto.
+       }   
+      }
+    }
+    
+    intros u1 u2 H3.
+    destruct u1; simpl in *; try intuition.
+    destruct u2; simpl in *; try intuition.
+    specialize (H0 a b).
+    unfold RAns_eq in H0.
+    assert (True /\ (forall h : A = B, b = eq_rect A id a B h)) as K1.
+    { split; auto.
+      intro hh.
+      dependent destruction hh; simpl.
+      dependent destruction H3. auto.
+    }  
+    specialize (H0 K1); pclearbot.
+    gstep; red.
+    econstructor.
+    gfinal; left.
+    eapply CIH; eauto.
+  }
+
+  { intros t0 t2 H0 H1; simpl.
+    setoid_rewrite interp_exec_tau.
+    setoid_rewrite tau_euttge.
+    setoid_rewrite (itree_eta t1).
+    eapply IHruttF; eauto.
+  }
+
+  { intros t1 t0 H1 H2; simpl.
+    setoid_rewrite interp_exec_tau.
+    setoid_rewrite tau_euttge.
+    setoid_rewrite (itree_eta t2).
+    eapply IHruttF; eauto.
+  }
+Qed.  
+
+Lemma lutt_absurd V1 (RR: V1 -> V1 -> Prop)
+               B (e : ErrEvent B) (k1 : B -> itree (ErrEvent +' E) V1) :
+  forall t1' : itree (ErrEvent +' E) V1,
+      rutt (REv_eq (fun (T : Type) (e : (ErrEvent +' E) T) => ~~ is_inlB e))
+        (RAns_eq (fun T : Type => fun=> TrueP)) RR 
+        (Vis (inl1 e) k1) t1' -> False.
+Proof.
+  intros.
+  punfold H; red in H.
+  dependent induction H.
+  { destruct H; simpl; intuition. }
+  eapply IHruttF; try reflexivity.
+Qed.
+
+(* inversion lemma? (2b generalized 2b useful):
+Lemma aux1 V1 (RR: V1 -> V1 -> Prop) :
+     forall t0 : itree (ErrEvent +' E) V1,
+      rutt (REv_eq (fun (T : Type) (e : (ErrEvent +' E) T) => ~~ is_inlB e))
+        (RAns_eq (fun T : Type => fun=> TrueP)) RR 
+        (Vis (inr1 e) k1) t0 ->
+    exists t1' : itree (ErrEvent +' E) V1,
+      rutt (REv_eq (fun (T : Type) (e0 : (ErrEvent +' E) T) => ~~ is_inlB e0))
+        (RAns_eq (fun T : Type => fun=> TrueP)) RR (k1 a) t1'.
+*)
+
+Lemma lutt2rutt_gen V1 (t1 t2: itree (ErrEvent +' E) V1) RR :
+  (*  @safe _ is_inlB V1 t1 -> *)
+  (exists t1', rutt
+       (REv_eq (fun (T : Type) (e : (ErrEvent +' E) T) => ~~ is_inlB e))
+       (RAns_eq (fun T : Type => fun=> TrueP)) RR t1 t1') ->
+  simple_rutt RR t1 t2 ->
+  rutt (REv_eq (fun (T : Type) (e : (ErrEvent +' E) T) => ~~ is_inlB e))
+       (RAns_eq (fun T : Type => fun=> TrueP)) RR t1 t2.            
+Proof.
+  revert t1 t2.
+  ginit. gcofix CIH.
+  intros t1 t2 H H0.
+  setoid_rewrite (itree_eta t1) in H.
+  setoid_rewrite (itree_eta t1).
+  setoid_rewrite (itree_eta t2).
+  punfold H0; red in H0.
+  remember (observe t1) as ot1.
+  remember (observe t2) as ot2.
+  simpl in H0.
+  hinduction H0 before CIH.
+  { intros t1 t2 H0 H1 H2.
+    gstep; red.
+    econstructor; auto.
+  }
+  { intros t1 t2 H0 H1 H2; pclearbot.
+    gstep; red.
+    econstructor.
+    gfinal; left.
+    eapply CIH; auto.
+    setoid_rewrite tau_euttge in H1; auto.
+  }
+  { intros t1 t2 H1 H2 H3.
+    gstep; red.    
+    destruct H as [hh H].
+    dependent destruction hh; simpl in *.
+    inv H.
+    destruct e2; simpl.
+    assert (False).
+    { destruct H2 as [t1' H2].
+      eapply lutt_absurd; eauto. }
+    intuition.
+    
+    econstructor; auto.
+    { unfold REv_eq; simpl.
+      split; eauto.
+      exists erefl; simpl; auto.
+    }
+
+    { intros a b H4.
+      gfinal; left.
+      eapply CIH; eauto.
+
+      { (* prove inversion lemma instead *)
+        destruct H2 as [t0 H2].
+        eapply rutt_inv_Vis_l in H2.
+        destruct H2 as [U3 [e3 [k3 [H2 [H5 H6]]]]].
+        destruct H5 as [_ [hh H5]]; simpl in *.
+        dependent destruction hh; simpl in *.
+        inv H5.
+        destruct H4 as [_ H4].
+        specialize (H4 erefl); simpl in *.
+        inv H4.
+        assert (RAns_eq (fun T : Type => fun=> TrueP)
+                  (@inr1 ErrEvent E _ e) a (inr1 e) a) as K.
+        { split; auto.
+          intros hh.
+          dependent destruction hh; simpl; auto.
+        }  
+        specialize (H6 a a K).
+        exists (k3 a); auto.
+      }  
+        
+      { destruct H4 as [_ H4].
+        specialize (H4 erefl); simpl in H4.
+        inv H4.
+        assert (a ~= a) as K.
+        { auto. }
+        specialize (H0 a a K); pclearbot; auto.
+      }
+    }
+  }
+
+  { intros t0 t2 H1 H2; simpl.
+    setoid_rewrite tau_euttge.
+    setoid_rewrite (itree_eta t1).
+    eapply IHruttF; eauto.
+    setoid_rewrite tau_euttge in H2.
+    setoid_rewrite (itree_eta t1) in H2; auto.
+  }
+  { intros t1 t0 H1 H2 H3; simpl.
+    setoid_rewrite tau_euttge.
+    setoid_rewrite (itree_eta t2).
+    eapply IHruttF; eauto.
+  }
+Qed.
+
+Lemma lutt2rutt V1 (t1 t2: itree (ErrEvent +' E) V1) RR :
+  (*  @safe _ is_inlB V1 t1 -> *)
+  (exists t1', rutt
+       (REv_eq (fun (T : Type) (e : (ErrEvent +' E) T) => ~~ is_inlB e))
+       (RAns_eq (fun T : Type => fun=> TrueP)) (R_eq TrueP) t1 t1') ->
+  simple_rutt RR t1 t2 ->
+  rutt (REv_eq (fun (T : Type) (e : (ErrEvent +' E) T) => ~~ is_inlB e))
+       (RAns_eq (fun T : Type => fun=> TrueP)) RR t1 t2.            
+Proof.
+  revert t1 t2.
+  ginit. gcofix CIH.
+  intros t1 t2 H H0.
+  setoid_rewrite (itree_eta t1) in H.
+  setoid_rewrite (itree_eta t1).
+  setoid_rewrite (itree_eta t2).
+  punfold H0; red in H0.
+  remember (observe t1) as ot1.
+  remember (observe t2) as ot2.
+  simpl in H0.
+  hinduction H0 before CIH.
+  { intros t1 t2 H0 H1 H2.
+    gstep; red.
+    econstructor; auto.
+  }
+  { intros t1 t2 H0 H1 H2; pclearbot.
+    gstep; red.
+    econstructor.
+    gfinal; left.
+    eapply CIH; auto.
+    setoid_rewrite tau_euttge in H1; auto.
+  }
+  { intros t1 t2 H1 H2 H3.
+    gstep; red.    
+    destruct H as [hh H].
+    dependent destruction hh; simpl in *.
+    inv H.
+    destruct e2; simpl.
+    assert (False).
+    { destruct H2 as [t1' H2].
+      eapply lutt_absurd; eauto. }
+    intuition.
+    
+    econstructor; auto.
+    { unfold REv_eq; simpl.
+      split; eauto.
+      exists erefl; simpl; auto.
+    }
+
+    { intros a b H4.
+      gfinal; left.
+      eapply CIH; eauto.
+
+      { (* prove inversion lemma instead *)
+        destruct H2 as [t0 H2].
+        eapply rutt_inv_Vis_l in H2.
+        destruct H2 as [U3 [e3 [k3 [H2 [H5 H6]]]]].
+        destruct H5 as [_ [hh H5]]; simpl in *.
+        dependent destruction hh; simpl in *.
+        inv H5.
+        destruct H4 as [_ H4].
+        specialize (H4 erefl); simpl in *.
+        inv H4.
+        assert (RAns_eq (fun T : Type => fun=> TrueP)
+                  (@inr1 ErrEvent E _ e) a (inr1 e) a) as K.
+        { split; auto.
+          intros hh.
+          dependent destruction hh; simpl; auto.
+        }  
+        specialize (H6 a a K).
+        exists (k3 a); auto.
+      }  
+        
+      { destruct H4 as [_ H4].
+        specialize (H4 erefl); simpl in H4.
+        inv H4.
+        assert (a ~= a) as K.
+        { auto. }
+        specialize (H0 a a K); pclearbot; auto.
+      }
+    }
+  }
+
+  { intros t0 t2 H1 H2; simpl.
+    setoid_rewrite tau_euttge.
+    setoid_rewrite (itree_eta t1).
+    eapply IHruttF; eauto.
+    setoid_rewrite tau_euttge in H2.
+    setoid_rewrite (itree_eta t1) in H2; auto.
+  }
+  { intros t1 t0 H1 H2 H3; simpl.
+    setoid_rewrite tau_euttge.
+    setoid_rewrite (itree_eta t2).
+    eapply IHruttF; eauto.
+  }
+Qed.
+
+
+Lemma test2_gen V1 d1 d2 
+  (t1: itree (ErrEvent +' E) V1) (t2: itree (ErrEvent +' E) V1) RR :
+  @safe _ is_inlB V1 t1 -> 
+  simple_rutt RR t1 t2 ->
+  simple_rutt RR (ret_dflt d1 t1) (ret_dflt d2 t2).
+Proof.
+  unfold safe, lutt.
+  intros H H0.
+  eapply test2_gen_ok2; eauto.
+  eapply rutt2ok_rutt.
+  eapply lutt2rutt; eauto.
+Qed.  
+ 
 
 End Test.
 
